In progress of completing skipped proof

PolarCodes/repeat_channelScript.sml
@@ -13,6 +13,9 @@ val _ = hide "W";
 (* TODO: find this definition somewhere                                       *)
 (* Probably apply general_cross from martingaleTheory?                        *)
 (*                                                                            *)
+(* TODO: redefine this as                                                     *)
+(*                                                                            *)
+(*                                                                            *)
 (* See {xs | LENGTH xs = n ∧ EVERY (combin$C (IN) (mcdomain0 W)) xs}. This    *)
 (* how it's defined in repeatChannel. If this is different, probably also     *)
 (* change it there.                                                           *)
@@ -21,8 +24,18 @@ val _ = hide "W";
 (* the output, no more, and no less.                                          *)
 (* -------------------------------------------------------------------------- *)
 Definition TODO_prod_set_def:
-  TODO_prod_set (set : α -> bool) (num_prod : num) = ARB : α list -> bool
+  TODO_prod_set (set : α -> bool) (num_prod : num) =
+  {xs | LENGTH xs = num_prod ∧
+        EVERY (combin$C (IN) set) xs} : α list -> bool
 End
+
+(*
+Theorem TODO_prod_set_alt:
+  ∀set num_prod.
+    TODO_prod_set set num_prod =  xs | LENGTH xs = n ∧ EVERY (combin$C (IN) (mcdomain0 W)) xs}
+Proof
+QED
+*)
 
 (* -------------------------------------------------------------------------- *)
 (* TODO: the reason we need these definitions, and can't just use the         *)
@@ -56,25 +69,25 @@ Theorem wf_memoryless_channel_repeat_channel0:
     wf_memoryless_channel W ⇒
     wf_memoryless_channel (repeat_channel0 W n)
 Proof
-  rpt gen_tac
+  rpt gen_tac >> strip_tac
   >> namedCases_on ‘W’ ["channel_dom channel_func"]
-  >> simp[wf_memoryless_channel_def, mcdomain0_def, mcchannel0_def]
-  >> disch_tac
+  >> gvs[wf_memoryless_channel_def]
   >> conj_tac
   (* Each input is mapped to a probability distribution *)
   >- (gen_tac
-      >> simp[repeat_channel0_def, mcchannel0_def]
+      >> gvs[repeat_channel0_def, mcchannel0_def, mcdomain0_def]
       >> strip_tac
       >> irule prob_space_pi_measure_space_list
       >> simp[ALL_EL_MAP]
       >> simp[EVERY_MEM]
       >> gen_tac >> strip_tac
       >> last_x_assum (fn th => irule (cj 1 th))
-      >> cheat
-     (*>> gvs[EVERY_MEM]
+      >> gvs[TODO_prod_set_def]
+      >> gvs[EVERY_MEM]
       >> last_x_assum dxrule
-      >> simp[mcdomain0_def]*)
+      >> simp[mcdomain0_def]
      )
+  (* Each probability distribution has the same sample space and sigma algebra *)
   >> rpt gen_tac >> strip_tac
   >> simp[repeat_channel0_def, mcchannel0_def]
   >> cheat
